$$
\begin{cases} x=x'+ut\\ y=y'\\ z=z'\\ t=t' \end{cases}
$$

$$
v=v'+u
$$

$$
\sum \vec{F_i} =m\frac{\mathrm{d} \vec{v} }{\mathrm{d} t} =0
$$

$$
\vec{F} =\frac{\mathrm{d} \vec{p} }{\mathrm{d} t} 
$$

$$
\vec{F}=\frac{\mathrm{d} m}{\mathrm{~d} t} \vec{v}+m \frac{\mathrm{d} \vec{v}}{\mathrm{~d} t}=\frac{\mathrm{d} m}{\mathrm{~d} t} \vec{v}+m \vec{a}=\frac{\mathrm{d} m}{\mathrm{~d} t} \vec{v}+m \frac{\mathrm{d}^{2} \vec{r}}{\mathrm{~d} t^{2}}
$$

$$
\vec{F}_{12}=-\vec{F}_{21}
$$

$$
\left\{\begin{array}{l} \nabla \cdot \boldsymbol{D}=\rho_{0} \\ \nabla \times \boldsymbol{E}=-\frac{\partial \boldsymbol{B}}{\partial t} \\ \nabla \cdot \boldsymbol{B}=0 \\ \nabla \times \boldsymbol{H}=\boldsymbol{j}_{0}+\frac{\partial \boldsymbol{D}}{\partial t} \end{array}\right.
$$

$$
c=\frac{1}{\sqrt{\mu_{0} \varepsilon_{0}}}
$$

$$
\begin{cases} x=x'+ut'\\ x'=x-ut \end{cases}
$$

$$
\begin{cases} x=\gamma (x'+ut')\\ x'=\gamma (x-ut) \end{cases}\tag 1
$$

$$
\begin{cases} x=ct\\ x'=ct' \end{cases}\tag 2
$$

$$
x^{\prime 2}+y^{\prime 2}+z^{\prime 2}-c^{2} t^{\prime 2}=x^{2}+y^{2}+z^{2}-c^{2}= t^{2}=0\tag 3
$$

$$
\begin{align} ctct' &amp; = \gamma^2(ct'+ut')(ct-ut)\\ ctct' &amp; = \gamma^2(c^2-u^2)tt'\\ c^2 &amp; = \gamma^2(c^2-u^2)\\ \end{align}
$$

$$
\gamma=\frac{1}{\sqrt{1-(\frac{u}{c})^2} } 
$$

$$
x'=\gamma (x-ut)
$$

$$
\begin{align} x &amp; = \gamma (x'+ut')\\ x &amp; = \gamma (\gamma (x-ut)+ut')\\ x &amp; =\gamma ^2 x-\gamma^2 ut+\gamma ut'\\ t'&amp; =\frac{1-\gamma ^2}{\gamma u} x+\gamma t\\ t'&amp; =\gamma(t+\frac{1-\gamma ^2}{\gamma ^2 u}x)\\ t'&amp; =\gamma(t+\frac{\frac{\frac{u^2}{c^2}}{1-\frac{u^2}{c^2}}}{\frac{1}{1-\frac{u^2}{c^2}}u}x)\\ t'&amp; =\gamma(t+\frac{u}{c^2}x) \end{align}
$$

$$
\left(\begin{array}{c} x^{\prime} \\ ct^{\prime} \end{array}\right)=\left(\begin{array}{cccc} \gamma &amp; -\gamma u / c  \\ -\gamma u / c &amp; \gamma   \end{array}\right)\left(\begin{array}{c} x \\ ct  \end{array}\right)
$$

$$
\left(\begin{array}{c} x \\ ct \end{array}\right)=\left(\begin{array}{cccc} \gamma &amp; \gamma u / c  \\ \gamma u / c &amp; \gamma   \end{array}\right)\left(\begin{array}{c} x^{\prime} \\ ct^{\prime}  \end{array}\right)
$$

$$
\left(\begin{array}{c} \Delta x^{\prime} \\ c\Delta t^{\prime} \end{array}\right)=\left(\begin{array}{cccc} \gamma &amp; -\gamma u / c  \\ -\gamma u / c &amp; \gamma   \end{array}\right)\left(\begin{array}{c} \Delta x \\ c\Delta t  \end{array}\right)
$$

$$
\begin{align} \left | A \right | &amp; = \gamma ^2-\frac{u^2}{c^2} \gamma ^2\\ &amp;=\gamma ^2(1-\frac{u^2}{c^2} )\\ &amp;=1 \end{align}
$$

$$
\left(\begin{array}{c} x^{\prime} \\ ct^{\prime} \end{array}\right)=\left(\begin{array}{cccc} cos\alpha  &amp; isin\alpha  \\ isin\alpha  &amp; cos\alpha   \end{array}\right)\left(\begin{array}{c} x \\ ct  \end{array}\right)
$$

$$
\begin{align} \left(\begin{array}{c} x \\ ct \end{array}\right) &amp; = \gamma\left(\begin{array}{cccc} 1 &amp;  u / c  \\  u / c &amp; 1   \end{array}\right)\left(\begin{array}{c} x^{\prime} \\ ct^{\prime} \end{array}\right)\\ &amp;=\gamma\left(\begin{array}{cccc} 1 &amp;  u / c  \\  u / c &amp; 1   \end{array}\right)\left(\begin{array}{c} 0 \\ c \end{array}\right)\\ &amp;=\gamma\left(\begin{array}{c} u \\ c \end{array}\right) \end{align} 
$$

$$
\begin{align} x&amp;=\gamma u(h)\\ t_1 &amp; = \gamma (h) \end{align}
$$

$$
\begin{align} t_2 &amp; = \frac{x}{c}\\ &amp;=\frac{\gamma u}{c} \end{align}
$$

$$
\begin{align} t&amp;=t_1+t_2\\ &amp; = \gamma + \gamma \frac{v}{c} \\ &amp;=\frac{1}{\sqrt{(1-\frac{v^2}{c^2}})} (1+\frac{v}{c})\\ &amp;=\sqrt{\frac{c+v}{c-v}}(h) \end{align}
$$

$$
\begin{align} \Delta t' &amp; = \gamma (\Delta t - \frac{u}{c^2}\Delta x)\\ &amp;=\gamma \Delta t\\ &amp;=\frac{\Delta t}{\sqrt{1-(\frac{v}{c})^2}}\\ &amp;=\frac{\Delta t}{\sqrt{1-(\frac{500}{3 \times 10^8})^2}} \end{align}
$$

$$
\begin{align} \Delta t' &amp; = \gamma (\Delta t - \frac{u}{c^2}\Delta x)\\ &amp;=\gamma \Delta t\\ &amp;=\frac{2.197\times 10^{-16}}{\sqrt{1-(\frac{0.99}{c})^2}} \end{align}
$$

$$
\begin{align} l&amp;=v\Delta t' \\ &amp;=0.99c \times \frac{2.197\times 10^{-16}}{\sqrt{1-(\frac{0.99c}{c})^2}}\\ &amp;=4.6\times 10 ^3 m \end{align}
$$

